Pop/Program.lean
@@ -4,11 +4,14 @@ import Pop.Pop
 import Pop.Util
 import Std.Data
 open Std.HashMap
-open Util Pop
+open Util
 
+namespace Pop
+
+-- TODO: Add values to writes
 def mkRequest : String × Address → ThreadId → Option Transition
   | ("R", addr), thId  => some $ Pop.Transition.acceptRequest (Pop.mkRead addr) thId
-  | ("W", addr), thId  => some $ Pop.Transition.acceptRequest (Pop.mkRead addr) thId
+  | ("W", addr), thId  => some $ Pop.Transition.acceptRequest (Pop.mkWrite addr) thId
   | ("Fence", _), thId => some $ Pop.Transition.acceptRequest (Pop.mkBarrier) thId
   | _, _ => none
 
@@ -52,3 +55,68 @@ macro_rules
   | `(request_set| $r:request_seq || $rs:request_set) => `($r :: $rs)
 macro_rules
   | `(<| $r |>) => `( createAcceptList $r)
+
+def Request.possiblePropagateTransitions (req : Request) (state :  SystemState) : List Transition :=
+  let threads := state.system.threads.removeAll req.propagated_to
+  --dbg_trace s!"Req {req.id} has not propagated to {threads}"
+  let threads_valid := threads.filter (state.canPropagate req.id)
+  --dbg_trace s!"Req {req.id} can propagate to {threads_valid}"
+  threads_valid.map λ th => Transition.propagateToThread req.id th
+
+def SystemState.possiblePropagateTransitions (state :  SystemState) : List Transition :=
+  let requests := filterNones state.requests.val.toList
+  let requests_not_fully_propagated := requests.filter λ r => ! (@Request.fullyPropagated state.system.scopes r state.system.scopes.systemScope)
+  let requests_active := requests_not_fully_propagated.filter λ r => (state.seen.elem r.id) && (!state.removed.elem r.id)
+  -- dbg_trace s!"active requests: {requests_active}"
+  List.join $ requests_active.map λ r => r.possiblePropagateTransitions state
+
+def Request.possibleSatisfyTransitions (read : Request) (state : SystemState) : List Transition :=
+  if !read.isRead then [] else
+    let requests := filterNones state.requests.val.toList
+    let writes_propagated_eq := requests.filter λ write => write.isWrite && write.propagated_to == read.propagated_to
+    let write_ids := writes_propagated_eq.map Request.id
+    let writes_valid := write_ids.filter (λ write => state.canSatisfyRead read.id write)
+    writes_valid.map $ Transition.satisfyRead read.id
+
+def SystemState.possibleSatisfyTransitions (state :  SystemState) : List Transition :=
+  let requests := filterNones state.requests.val.toList
+  let unsatisfied_reads := requests.filter λ r => r.isRead && !(state.isSatisfied r.id)
+  List.join $ unsatisfied_reads.map λ r => r.possibleSatisfyTransitions state
+
+def SystemState.possibleTransitions (state : SystemState) (unaccepted : List Transition) :=
+  let accepts := unaccepted.filter Transition.isAccept
+  accepts ++ state.possibleSatisfyTransitions ++ state.possiblePropagateTransitions
+
+-- This should be a monad transformer or smth...
+def SystemState.takeNthStep (state : SystemState) (acceptRequests : List Transition) (n : Nat) : Except String (Transition × SystemState) :=
+  let transitions := state.possibleTransitions acceptRequests
+  --dbg_trace s!"possible transitions: {transitions}"
+  if transitions.isEmpty then
+    throw "No more transitions possible"
+  else
+    let opTrans := transitions.get? (n.mod transitions.length)
+    match opTrans with
+      | none => unreachable!
+      | some trans => Except.map (λ st => (trans, st)) (state.applyTransition trans)
+
+def SystemState._runWithList  : SystemState →  List Transition → List Nat → Except String SystemState
+  | state, accepts, ns => match ns with
+    | [] => throw "Empty transition number list"
+    | n::ns =>
+      let runStep := state.takeNthStep accepts n
+      match runStep with
+        | Except.error "No more transitions possible" => Except.ok state
+        | Except.ok (trans,state') =>
+          dbg_trace trans.toString
+          dbg_trace state'
+          state'._runWithList (accepts.removeAll [trans]) ns
+        | Except.error e => Except.error e
+
+def SystemState.runWithList  : SystemState →  List Transition → List Nat → Except String SystemState
+  | state, accepts, ns => if !accepts.all Transition.isAccept
+  then throw "Running with non-accept transition inputs"
+  else SystemState._runWithList state accepts ns
+
+    -- let runStep := λ (acceptsRemaining, state) n => state.takeNthStep acceptsRemaining n
+    -- ns.foldlM (init := (accepts, state)) runStep
+    -- ns.foldlM  (init := state) λ state.takeNthStep accepts.zip ns 
