Pop/Test.lean
@@ -7,12 +7,12 @@ namespace Test
 open Util Pop
 
 
-theorem proof1 : List.sublist [1] [1,2] := by simp
-theorem proof2 : List.sublist [2] [1,2] := by simp
+theorem proof1 : List.sublist [0] [0,1] := by simp
+theorem proof2 : List.sublist [1] [0,1] := by simp
 open ListTree in
-def scopes12 : ListTree ThreadId [1,2] :=  parentCons (ListTree.leaf [2]) (parentCons (ListTree.leaf [1]) (parentNil [1,2]) proof1) proof2
+def scopes12 : ListTree ThreadId [0,1] :=  parentCons (ListTree.leaf [1]) (parentCons (ListTree.leaf [0]) (parentNil [0,1]) proof1) proof2
 
-def valid_scopes12 : ValidScopes := { system_scope := [1,2], scopes := scopes12, threads_in := sorry}
+def valid_scopes12 : ValidScopes := { system_scope := [0,1], scopes := scopes12, threads_in := sorry}
 
 def tso_reorder : Request → Request → Bool
   | r₁, r₂ => if r₁.isBarrier || r₂.isBarrier
@@ -26,16 +26,30 @@ def tso12 : System := { scopes := valid_scopes12, reorder_condition := tso_reord
 
 def inittso12 : SystemState := SystemState.init tso12
 
-open Transition 
+open Transition
 
 def trace := [acceptRequest (mkRead 0) 0, acceptRequest (mkWrite 0) 0]
 def trace2 := [acceptRequest (mkRead 0) 0, acceptRequest (mkWrite 0) 1, propagateToThread 0 1, propagateToThread 1 0, satisfyRead 0 1]
 
-def res := printResult $ inittso12.applyTrace trace
-def res2 := printResult $ inittso12.applyTrace trace2
+-- def res := printResult $ inittso12.applyTrace trace
+-- def res2 := printResult $ inittso12.applyTrace trace2
 
 
 def testprogram := <| R x || W y ; W x|>
 #eval testprogram.toString
+
+
+def testaccept := inittso12.acceptRequest (mkRead 0) 0
+#eval testaccept.canPropagate 0 1 
+#eval testaccept.requests.val[0]
+#eval testaccept.requests.val[0].get!.isPropagated 1
+    -- let scope := testaccept.system.scopes.jointScope 0 req.thread
+    -- let pred := testaccept.orderConstraints.predecessors scope 0 (reqIds testaccept.requests)
+    -- let reqOps := testaccept.requests.val.filter (λ req => match req with | none => false | some r => pred.elem r.id)
+    -- let reqs := filterNones reqOps.toList
+    -- let predPropagated := reqs.map (λ r => r.fullyPropagated state.system.scopes.systemScope)
+    -- unpropagated || predPropagated.foldl (. && .) true
+-- #eval inittso12.system.threads
+--#eval testaccept.toOption.get!.canPropagate 0 1
 
 end Test
